BinaryHeap/Basic.lean
@@ -1,0 +1,61 @@
+/-
+  This file contains the Binary Heap type and its basic operations.
+-/
+import BinaryHeap.CompleteTree
+
+abbrev BinaryHeap.TotalAndTransitiveLe (le : α → α → Bool) : Prop := BinaryHeap.transitive_le le ∧ BinaryHeap.total_le le
+
+structure BinaryHeap (α : Type u) (le : α → α → Bool) (n : Nat) where
+  tree : BinaryHeap.CompleteTree α n
+  valid : BinaryHeap.HeapPredicate tree le
+  wellDefinedLe : BinaryHeap.TotalAndTransitiveLe le
+deriving Repr
+
+namespace BinaryHeap
+
+/-- Creates an empty heap. O(1) -/
+def new {α : Type u} {le : α → α → Bool} (h₁ : TotalAndTransitiveLe le) : BinaryHeap α le 0 :=
+  {
+    tree := CompleteTree.empty,
+    valid := CompleteTree.emptyIsHeap le
+    wellDefinedLe := h₁
+  }
+
+/-- Adds an element into a heap. O(log(n)) -/
+def push {α : Type u} {le : α → α → Bool} {n : Nat} : α → BinaryHeap α le n → BinaryHeap α le (n+1)
+| elem, .mk tree valid wellDefinedLe =>
+  let valid := tree.heapPushIsHeap valid wellDefinedLe.left wellDefinedLe.right
+  let tree := tree.heapPush le elem
+  {tree, valid, wellDefinedLe}
+
+/-- Removes the smallest element from the heap and returns it. O(log(n)) -/
+def pop {α : Type u} {le : α → α → Bool} {n : Nat} : (BinaryHeap α le (n+1)) → (α × BinaryHeap α le n)
+| {tree, valid, wellDefinedLe} =>
+  let result := tree.heapPop le
+  let resultValid := CompleteTree.heapPopIsHeap le tree valid wellDefinedLe
+  (result.fst, { tree := result.snd, valid := resultValid, wellDefinedLe})
+
+/-- Removes the element at the given (depth-first) index from the heap and returns it. O(log(n)) -/
+def removeAt {α : Type u} {le : α → α → Bool} {n : Nat} : (BinaryHeap α le (n+1)) → (Fin (n+1)) → (α × BinaryHeap α le n)
+| {tree, valid, wellDefinedLe}, index =>
+  let result := tree.heapRemoveAt le index
+  let resultValid := CompleteTree.heapRemoveAtIsHeap le index tree valid wellDefinedLe
+  (result.fst, { tree := result.snd, valid := resultValid, wellDefinedLe})
+
+/-- Updates the element at the given (depth-first) index and returns its previous value. O(log(n)) -/
+def updateAt {α : Type u} {le : α → α → Bool} {n : Nat} : (BinaryHeap α le n) → (Fin n) → α → (BinaryHeap α le n × α)
+| {tree, valid, wellDefinedLe}, index, value =>
+  let result := tree.heapUpdateAt le index value
+  let resultValid := CompleteTree.heapUpdateAtIsHeap le index value tree valid wellDefinedLe.left wellDefinedLe.right
+  ({ tree := result.fst, valid := resultValid, wellDefinedLe}, result.snd)
+
+/-- Searches for an element in the heap and returns its index. **O(n)** -/
+def indexOf {α : Type u} {le : α → α → Bool} {n : Nat} : BinaryHeap α le n → (pred : α → Bool) → Option (Fin n)
+| {tree, valid := _, wellDefinedLe := _}, pred =>
+  tree.indexOf pred
+
+instance : GetElem (BinaryHeap α le n) (Nat) α (λ _ index ↦ index < n) where
+  getElem := λ heap index h₁ ↦ heap.tree.get ⟨index, h₁⟩
+
+instance : GetElem (BinaryHeap α le n) (Fin n) α (λ _ _ ↦ True) where
+  getElem := λ heap index _ ↦ heap.tree.get index
