BinaryHeap/CompleteTree/HeapProofs/HeapPop.lean
@@ -3,7 +3,7 @@ import BinaryHeap.CompleteTree.HeapProofs.HeapUpdateRoot
 
 namespace BinaryHeap.CompleteTree
 
-theorem heapPopIsHeap {α : Type u} {n : Nat} (le : α → α → Bool) (heap : CompleteTree α (n+1)) (h₁ : HeapPredicate heap le) (wellDefinedLe : transitive_le le ∧ total_le le) : HeapPredicate (heap.heapPop le).fst le := by
+theorem heapPopIsHeap {α : Type u} {n : Nat} (le : α → α → Bool) (heap : CompleteTree α (n+1)) (h₁ : HeapPredicate heap le) (wellDefinedLe : transitive_le le ∧ total_le le) : HeapPredicate (heap.heapPop le).snd le := by
   have h₂ : HeapPredicate (Internal.heapRemoveLast heap).fst le := CompleteTree.heapRemoveLastIsHeap h₁ wellDefinedLe.left wellDefinedLe.right
-  unfold heapPop
+  unfold heapPop heapPop.Prod.swap
   cases n <;> simp[h₂, heapUpdateRootIsHeap, wellDefinedLe]
