BinaryHeap/CompleteTree/HeapProofs/HeapRemoveAt.lean
@@ -3,7 +3,7 @@ import BinaryHeap.CompleteTree.HeapProofs.HeapUpdateAt
 
 namespace BinaryHeap.CompleteTree
 
-theorem heapRemoveAtIsHeap {α : Type u} {n : Nat} (le : α → α → Bool) (index : Fin (n+1)) (heap : CompleteTree α (n+1)) (h₁ : HeapPredicate heap le) (wellDefinedLe : transitive_le le ∧ total_le le) : HeapPredicate (heap.heapRemoveAt le index).fst le := by
+theorem heapRemoveAtIsHeap {α : Type u} {n : Nat} (le : α → α → Bool) (index : Fin (n+1)) (heap : CompleteTree α (n+1)) (h₁ : HeapPredicate heap le) (wellDefinedLe : transitive_le le ∧ total_le le) : HeapPredicate (heap.heapRemoveAt le index).snd le := by
   have h₂ : HeapPredicate (Internal.heapRemoveLastWithIndex heap).fst le := CompleteTree.heapRemoveLastWithIndexIsHeap h₁ wellDefinedLe.left wellDefinedLe.right
   unfold heapRemoveAt
   split
