BinaryHeap/Relations.lean
@@ -1,0 +1,19 @@
+/-
+  This file contains proofs for relations that might be helpful for creating heaps.
+ -/
+import BinaryHeap.HeapPredicate
+
+namespace BinaryHeap
+
+/--Helper for the common case of using natural numbers for sorting.-/
+theorem nat_ble_to_heap_le_total : total_le Nat.ble :=
+  λa b ↦ Nat.ble_eq.substr $ Nat.ble_eq.substr (Nat.le_total a b)
+
+/--Helper for the common case of using natural numbers for sorting.-/
+theorem nat_ble_to_heap_transitive_le : transitive_le Nat.ble :=
+  λ a b c ↦
+    Nat.le_trans (n := a) (m := b) (k := c)
+    |> Nat.ble_eq.substr
+    |> Nat.ble_eq.substr
+    |> Nat.ble_eq.substr
+    |> and_imp.mpr
